\documentclass[]{article}
\usepackage{lmodern}
\usepackage{amssymb,amsmath}
\usepackage{ifxetex,ifluatex}
\usepackage{fixltx2e} % provides \textsubscript
\ifnum 0\ifxetex 1\fi\ifluatex 1\fi=0 % if pdftex
  \usepackage[T1]{fontenc}
  \usepackage[utf8]{inputenc}
\else % if luatex or xelatex
  \ifxetex
    \usepackage{mathspec}
  \else
    \usepackage{fontspec}
  \fi
  \defaultfontfeatures{Ligatures=TeX,Scale=MatchLowercase}
\fi
% use upquote if available, for straight quotes in verbatim environments
\IfFileExists{upquote.sty}{\usepackage{upquote}}{}
% use microtype if available
\IfFileExists{microtype.sty}{%
\usepackage[]{microtype}
\UseMicrotypeSet[protrusion]{basicmath} % disable protrusion for tt fonts
}{}
\PassOptionsToPackage{hyphens}{url} % url is loaded by hyperref
\usepackage[unicode=true]{hyperref}
\hypersetup{
            pdfborder={0 0 0},
            breaklinks=true}
\urlstyle{same}  % don't use monospace font for urls
\IfFileExists{parskip.sty}{%
\usepackage{parskip}
}{% else
\setlength{\parindent}{0pt}
\setlength{\parskip}{6pt plus 2pt minus 1pt}
}
\setlength{\emergencystretch}{3em}  % prevent overfull lines
\providecommand{\tightlist}{%
  \setlength{\itemsep}{0pt}\setlength{\parskip}{0pt}}
\setcounter{secnumdepth}{0}
% Redefines (sub)paragraphs to behave more like sections
\ifx\paragraph\undefined\else
\let\oldparagraph\paragraph
\renewcommand{\paragraph}[1]{\oldparagraph{#1}\mbox{}}
\fi
\ifx\subparagraph\undefined\else
\let\oldsubparagraph\subparagraph
\renewcommand{\subparagraph}[1]{\oldsubparagraph{#1}\mbox{}}
\fi

% set default figure placement to htbp
\makeatletter
\def\fps@figure{htbp}
\makeatother


\date{}

\begin{document}

\subsection{67}\label{header-n36}

记 \(Y\) 为长方形的高度, 依题意

\[E(Y | X)=\frac{X}{2}\\
E(X)=\frac{1}{2}\]

\subsection{周长}\label{header-n40}

\[E(2(X+Y))=2E(X+Y)\]

根据定理, 这等于

\[2E(X+Y)=2E(E(X+Y|X))\]

考虑 \(E(X+Y|X)\)

\[E(X+Y|X)=X+E(Y|X)=\frac{3X}{2}\]

所以周长的期望为

\[2E(\frac{3X}{2})=3E(X)=\frac{3}{2}\]

\subsection{面积}\label{header-n48}

\[E(XY)=E(E(XY|X))\]

考虑 \(E(XY|X)\)

\[E(XY|X)=XE(Y|X)=\frac{X^2}{2}\]

所以面积的期望为

\[E(XY)=E(\frac{X^2}{2})=\frac{1}{2}\int_0^1x^2dx=\frac{1}{6}\]

\section{77}\label{header-n54}

\subsection{a}\label{header-n55}

\subsubsection{协方差}\label{header-n67}

\[f_{X}(x)=\int_{x}^{+\infty} f(x, y) d y=\int_{x}^{+\infty} e^{-y} d y=-\left.e^{-y}\right|_{x} ^{+\infty}=e^{-x}\]

\[f_{Y}(y)=\int_{0}^{y} f(x, y) d x=\int_{0}^{y} e^{-y} d x=y \cdot e^{-y}\]

所以

\[E(X)=\int_{0}^{+\infty} x \cdot f_{X}(x) d x=\int_{0}^{+\infty} x \cdot e^{-x} d x=1\]

\[E(Y)=\int_{0}^{+\infty} y \cdot f_{Y}(y) d y=\int_{0}^{+\infty} y^{2} \cdot e^{-y} d y=2\]

又

\[E(X \cdot Y)=\int_{0}^{+\infty}\left(\int_{x}^{+\infty} x \cdot y \cdot f(x, y) d y\right) d x=\int_{0}^{+\infty}\left(\int_{x}^{+\infty} x \cdot y \cdot e^{-y} d y\right) d x=3\]

所以

\[\operatorname{Cov}(X, Y)=3-2 \cdot 1=1\]

\subsubsection{相关系数}\label{header-n64}

\[E\left(X^{2}\right)=\int_{0}^{+\infty} x^{2} \cdot f_{X}(x) d x=\int_{0}^{+\infty} x^{2} \cdot e^{-x} d x=2\]

\[E\left(Y^{2}\right)=\int_{0}^{+\infty} y^{2} \cdot f_{Y}(y) d y=\int_{0}^{+\infty} y^{3} \cdot e^{-y} d y=6\]

所以

\[\operatorname{Var}(X)=2-1^{2}=1\\
\operatorname{Var}(Y)=6-2^{2}=2\]

从而

\[\rho(X, Y)=\frac{1}{\sqrt{1 \cdot 2}}=\frac{\sqrt 2}{2}\]

\subsection{b}\label{header-n79}

\[f_{X | Y}(x | y)=\frac{f_{X, Y}(x, y)}{f_{Y}(y)}=\frac{e^{-y}}{y \cdot e^{-y}}=\frac{1}{y}\]

\[f_{Y | X}(y | x)=\frac{f_{X, Y}(x, y)}{f_{X}(x)}=\frac{e^{-y}}{e^{-x}}=e^{x-y}\]

所以

\[E(X | Y=y)=\int_{0}^{y} x \cdot f_{X | Y}(x | y) d x=\int_{0}^{y} x \cdot \frac{1}{y} d x=\frac{1}{y} \cdot \int_{0}^{y} x d x=\frac{y}{2}\]

\[E(Y | X=x)=\int_{x}^{+\infty} y \cdot f_{Y | X}(y | x) d y=\int_{x}^{+\infty} y \cdot e^{x-y} d y=x+1\]

\subsection{c}\label{header-n92}

令

\[U=E(X|Y)=\frac{Y}{2}\\
V=E(Y|X)=X+1\]

所以

\[f_U(u)=y(u) \cdot e^{-y(u)} \cdot y'(u)=4 ue^{-2 u} \quad u\ge0\]

\[f_V(v)=e^{-x(v)} \cdot x'(v)=e^{1-v}\quad v\ge1\]

\end{document}
