\documentclass[]{article}
\usepackage{lmodern}
\usepackage{amssymb,amsmath}
\usepackage{ifxetex,ifluatex}
\usepackage{fixltx2e} % provides \textsubscript
\ifnum 0\ifxetex 1\fi\ifluatex 1\fi=0 % if pdftex
  \usepackage[T1]{fontenc}
  \usepackage[utf8]{inputenc}
\else % if luatex or xelatex
  \ifxetex
    \usepackage{mathspec}
  \else
    \usepackage{fontspec}
  \fi
  \defaultfontfeatures{Ligatures=TeX,Scale=MatchLowercase}
\fi
% use upquote if available, for straight quotes in verbatim environments
\IfFileExists{upquote.sty}{\usepackage{upquote}}{}
% use microtype if available
\IfFileExists{microtype.sty}{%
\usepackage[]{microtype}
\UseMicrotypeSet[protrusion]{basicmath} % disable protrusion for tt fonts
}{}
\PassOptionsToPackage{hyphens}{url} % url is loaded by hyperref
\usepackage[unicode=true]{hyperref}
\hypersetup{
            pdfborder={0 0 0},
            breaklinks=true}
\urlstyle{same}  % don't use monospace font for urls
\IfFileExists{parskip.sty}{%
\usepackage{parskip}
}{% else
\setlength{\parindent}{0pt}
\setlength{\parskip}{6pt plus 2pt minus 1pt}
}
\setlength{\emergencystretch}{3em}  % prevent overfull lines
\providecommand{\tightlist}{%
  \setlength{\itemsep}{0pt}\setlength{\parskip}{0pt}}
\setcounter{secnumdepth}{0}
% Redefines (sub)paragraphs to behave more like sections
\ifx\paragraph\undefined\else
\let\oldparagraph\paragraph
\renewcommand{\paragraph}[1]{\oldparagraph{#1}\mbox{}}
\fi
\ifx\subparagraph\undefined\else
\let\oldsubparagraph\subparagraph
\renewcommand{\subparagraph}[1]{\oldsubparagraph{#1}\mbox{}}
\fi

% set default figure placement to htbp
\makeatletter
\def\fps@figure{htbp}
\makeatother


\date{}

\begin{document}

\section{54}\label{header-n0}

\[\operatorname{Cov}(U, V)=\operatorname{Cov}(Z+X, Z+Y)=\operatorname{Cov}(Z, Z)+\operatorname{Cov}(Z, Y)+\operatorname{Cov}(X, Z)+\operatorname{Cov}(X, Y)\]

分别计算得

\[\operatorname{Cov}(Z, Z)=\operatorname{Var}(Z)=\sigma_Z^2
\\
\operatorname{Cov}(Z, Y)=0
\\
\operatorname{Cov}(X, Z)=0
\\
\operatorname{Cov}(X, Y)=0\]

所以

\[\operatorname{Cov}(U, V)=\sigma_Z^2\]

相关系数为

\[\rho(U, V)=\frac{\operatorname{Cov}(U, V)}{\sqrt{\operatorname{Var}(U) \cdot \operatorname{Var}(V)}}\]

\[\operatorname{Var}(U)=\operatorname{Var}(Z+X)=\operatorname{Cov}(Z+X,Z+X)=\operatorname{Var}(Z)+\operatorname{Var}(X)+2 \cdot \operatorname{Cov}(Z, X)=\sigma_{X}^{2}+\sigma_{Z}^{2}\]

同理可得

\[\operatorname{Var}(V)=\operatorname{Var}(Z+Y)=\operatorname{Var}(Z)+\operatorname{Var}(Y)+2 \cdot \operatorname{Cov}(Z, Y)=\sigma_{Y}^{2}+\sigma_{Z}^{2}\]

代入得

\[\rho(U, V)=\frac{\sigma_{Z}^{2}}{\sqrt{\left(\sigma_{X}^{2}+\sigma_{Z}^{2}\right) \cdot\left(\sigma_{Y}^{2}+\sigma_{Z}^{2}\right)}}=\frac{1}{\sqrt{\left(1+\sigma_{X}^{2}\right) \cdot\left(1+\sigma_{Y}^{2}\right)}}\]

\section{60}\label{header-n14}

\[E(XY)=E(SY^2)=E(SY^2|S=1)P(S=1)+E(SY^2|S=-1)P(S=-1)=\frac{E(Y^2)+E(-Y^2)}{2}=0\]

\[E(SY)=E(SY|S=1)P(S=1)+E(SY|S=-1)P(S=-1)=\frac{E(Y)+E(-Y)}{2}=0\]

所以

\[\operatorname{Cov}(X, Y)=E(X \cdot Y)-E(X) \cdot E(Y)=E\left(S \cdot Y^{2}\right)-E(S \cdot Y) \cdot E(Y)=0-0=0\]

\[F_{X}(x)=P(X \leq x)=P(S \cdot Y \leq x)=\iint_{s \cdot y \leq x} f_{S, Y}(s, y) d s d y=\iint_{s \cdot y \leq x} f_{S}(s) \cdot f_{Y}(y) d s d y\]

注意到

\[P(S \cdot Y \leq x)=P(S \cdot Y \leq x|S=1)P(S=1)+P(S \cdot Y \leq x|S=-1)P(S=-1)\]

\[P(S \cdot Y \leq x|S=1)=P(Y\le x)=F_Y(x)\\
P(S \cdot Y \leq x|S=-1)=P(Y\ge -x)=1-F_Y(-x)\]

所以

\[F_{X}(x)=\frac{1}{2} \cdot\left(1-F_{Y}(-x)\right)+\frac{1}{2} \cdot F_{Y}(x)=\frac{1}{2} \cdot F_{Y}(x)-\frac{1}{2} \cdot F_{Y}(-x)+\frac{1}{2}\]

由于 Y 的密度函数关于 \(y\) 轴对称

\[f_{Y}(x)=f_{Y}(-x)\]

所以

\[f_{X}(x)=F_{X}^{\prime}(x)=\left(\frac{1}{2} \cdot F_{Y}(x)-\frac{1}{2} \cdot F_{Y}(-x)+\frac{1}{2}\right)^{\prime}=\frac{1}{2} \cdot f_{Y}(x)+\frac{1}{2} \cdot f_{Y}(-x)=f_Y(x)\]

然而

\[f_{X | Y}(x | y)=\left\{\begin{array}{ll}{\frac{1}{2},} & {x=\pm y} \\ {0,} & {\text { 其他 }}\end{array}\right.\]

所以

\[f_{X | Y}(x | y) \neq f_{X}(x)\]

这表明 \(X\) 和 \(Y\) 不独立

\section{补充题}\label{header-n34}

\subsection{1.}\label{header-n42}

\[E(X)=\int_{-\infty}^{\infty}xf(x) dx=\int_{-\infty}^{0}\frac{xe^{x}}{2} dx+\int_{0}^{\infty}\frac{xe^{-x}}{2} dx=\left.\frac{e^{x} (x-1)}{2}\right|_{-\infty}^{0}+\left.\frac{e^{-x} (-x-1)}{2}\right|_{0} ^{\infty}=-\frac{1}{2}+\frac{1}{2}=0\]

\[E(X^2)=\int_{-\infty}^{\infty}x^2f(x) dx=\int_{-\infty}^{0}\frac{x^2e^{x}}{2} dx+\int_{0}^{\infty}\frac{x^2e^{-x}}{2} dx=\\
\left.\frac{e^{x} (x^2-2 x+2)}{2}\right|_{-\infty}^{0}+\left.\frac{e^{-x} (-x^2-2 x-2)}{2}\right|_{0} ^{\infty}=1+1=2\]

所以

\[D(X)=E(X^2)-E(X)^2=2-0^2=2\]

\subsection{2.}\label{header-n46}

不独立, 考虑事件 \(X>1\) 和 \(|X|\ge1\)

\[P(X\ge1)=\int_1^{\infty } \frac{ e^{-x}}{2} \, dx=\frac{1}{2e}\]

\[P(|X|\ge1)=P(X \ge 1)+P(X \le -1)=\frac{1}{e}\]

而

\[P(X\ge 1,|X|\ge1)=P(X\ge1)=\frac{1}{2e}\neq P(X\ge 1)P(|X|\ge1)\]

\subsubsection{3.}\label{header-n66}

由于 \(X\) 和 \(|X|\) 不独立, 所以它们一定相关

\end{document}
